updated Spec.v to no longer have axioms vs ops

theories/Spec.v
@@ -80,31 +80,18 @@ Definition sats_op_pred {T} (p: OpPred T) : T -> Prop :=
 (* Allows writing "oppred t" instead of "sats_op_pred oppred t" *)
 Coercion sats_op_pred : OpPred >-> Funclass.
 
-(* The type of the representation of an axiom in a spec *)
-Inductive SpecAxiom : Type :=
-| specAxiom (f:Field) (P:Prop)
-.
-
-Arguments specAxiom f%string P%type.
-
-(* Projections of SpecAxiom *)
-Definition axiom_name (ax:SpecAxiom) :=
-  let (f,_) := ax in f.
-Definition axiom_prop (ax:SpecAxiom) :=
-  let (_,P) := ax in P.
-
 (* The inductive representation of specs, indexed by the op fields *)
 Inductive Spec : Type :=
-(* The base case contains the names and types of the axioms *)
-| Spec_Axioms (axioms : list SpecAxiom) : Spec
+(* The base case, which is the empty spec *)
+| Spec_Nil : Spec
 (* The inductive case adds an op named f with zero or more definitions to the
 rest of the spec, that can depend on any f equal to all the definitions *)
-| Spec_ConsOp (f:Field) (T : Type) (oppred: OpPred T)
-              (rest : forall t, oppred t -> Spec) : Spec
+| Spec_Cons (f:Field) (T : Type) (oppred: OpPred T)
+            (rest : forall t, oppred t -> Spec) : Spec
 .
 
 (* Make the field argument be parsed by Coq as a string *)
-Arguments Spec_ConsOp f%string T oppred rest.
+Arguments Spec_Cons f%string T oppred rest.
 
 (* Unfold a definition *)
 Definition def {T x} (t:T) (t__pf: t = x) : T := x.
@@ -112,67 +99,45 @@ Definition def {T x} (t:T) (t__pf: t = x) : T := x.
 
 (*** Models ***)
 
-(* Helper for conjoining all the axioms in an axiom list *)
-Fixpoint conjoin_axioms (axioms : list SpecAxiom) : Prop :=
-  match axioms with
-    | [] => True
-    | [specAxiom _ P] => P
-    | (specAxiom _ P) :: axioms' => P /\ conjoin_axioms axioms'
-  end.
+(* The type of models of Spec_Cons f T oppred rest, given the type U of models
+of rest *)
+Inductive ModelCons (T:Type) (oppred:OpPred T)
+          (U: forall t, oppred t -> Type) : Type :=
+| modelCons (t:T) (pf:oppred t) (model':U t pf)
+.
 
-(* Helper for proving conjoin_axioms applied to a cons *)
-Lemma conjoin_axioms_cons f (P:Prop) axioms :
-  P -> conjoin_axioms axioms -> conjoin_axioms (specAxiom f P :: axioms).
-  intros; destruct axioms; try split; assumption.
-Qed.
+Arguments modelCons {T oppred U} t pf model'.
 
-(* Helper for destructing conjoin_axioms applied to a cons *)
-Lemma conjoin_axioms_destruct f (P:Prop) axioms :
-  conjoin_axioms (specAxiom f P :: axioms) -> P /\ conjoin_axioms axioms.
-  intro H; destruct axioms; try (destruct H); split; try assumption; try constructor.
-Qed.
-
-(* Build the type of the op of a spec *)
-Fixpoint spec_ops spec : Type :=
+(* Build the type of the models of a spec *)
+Fixpoint spec_model spec : Type :=
   match spec with
-    | Spec_Axioms axioms => unit
-    | Spec_ConsOp f T oppred rest =>
-      { t : T & {pf: oppred t & spec_ops (rest t pf)}}
+    | Spec_Nil => unit
+    | Spec_Cons f T oppred rest =>
+      ModelCons T oppred (fun t pf => spec_model (rest t pf))
   end.
-
-(* Build the type of the models of spec as a nested dependent pair *)
-Fixpoint spec_model spec : spec_ops spec -> Prop :=
-  match spec return spec_ops spec -> Prop with
-    | Spec_Axioms axioms =>
-      fun _ => conjoin_axioms axioms
-    | Spec_ConsOp f T oppred rest =>
-      fun ops =>
-        spec_model (rest (projT1 ops) (projT1 (projT2 ops)))
-                   (projT2 (projT2 ops))
-  end.
-
-(* Build the ops for a spec from an op for the head and ops for the tail *)
-Definition ops_cons {f T} {oppred: OpPred T} {rest}
-           (t:T) (pf:oppred t) (ops_rest:spec_ops (rest t pf)) :
-  spec_ops (Spec_ConsOp f T oppred rest) :=
-  existT _ t (existT _ pf ops_rest).
 
 (* Project the first op of a spec *)
-Definition ops_head {f T oppred rest}
-           (ops: spec_ops (Spec_ConsOp f T oppred rest)) : T :=
-  projT1 ops.
+Definition model_head {f T oppred rest}
+           (model: spec_model (Spec_Cons f T oppred rest)) : T :=
+  match model with
+    | modelCons t pf model' => t
+  end.
 
 (* Project the proof that the first op of a spec meets its oppred *)
-Definition ops_proof {f T oppred rest}
-           (ops: spec_ops (Spec_ConsOp f T oppred rest)) :
-  oppred (ops_head ops) :=
-  projT1 (projT2 ops).
+Definition model_proof {f T oppred rest}
+           (model: spec_model (Spec_Cons f T oppred rest)) :
+  oppred (model_head model) :=
+  match model with
+    | modelCons t pf model' => pf
+  end.
 
-(* Project the tail of the ops of a spec *)
-Definition ops_rest {f T oppred rest}
-           (ops: spec_ops (Spec_ConsOp f T oppred rest)) :
-  spec_ops (rest (ops_head ops) (ops_proof ops)) :=
-  projT2 (projT2 ops).
+(* Project the tail of the model of a spec *)
+Definition model_rest {f T oppred rest}
+           (model: spec_model (Spec_Cons f T oppred rest)) :
+  spec_model (rest (model_head model) (model_proof model)) :=
+  match model with
+    | modelCons t pf model' => model'
+  end.
 
 
 (*** Spec Examples ***)
@@ -191,103 +156,134 @@ Notation "'Axioms f1 t1 ; .. ; fn tn'" :=
 
 (* Example 1:  op n:nat;  axiom gt1: n > 1 *)
 Definition spec_example_1 :=
-  Spec_ConsOp "n" nat Pred_Trivial
-              (fun n _ => Spec_Axioms [specAxiom "gt1" (n > 1)]).
+  Spec_Cons "n" nat Pred_Trivial
+              (fun n _ =>
+                 Spec_Cons "gt1" (n>1) Pred_Trivial
+                           (fun _ _ => Spec_Nil)).
 
 (* Example 2:  op n:nat := 2;  (no axioms) *)
 Definition spec_example_2 :=
-  Spec_ConsOp "n" nat (Pred_Eq 2)
-              (fun n _ => Spec_Axioms []).
+  Spec_Cons "n" nat (Pred_Eq 2)
+            (fun n _ => Spec_Nil).
 
 (* Example 3:  op T:Set := nat;  op n:T__def;  axiom gt1: n > 1 *)
 Definition spec_example_3 :=
-  Spec_ConsOp
+  Spec_Cons
     "T" Set (Pred_Eq nat)
     (fun T T__pf =>
-       Spec_ConsOp "n" (def T T__pf) Pred_Trivial
-                   (fun n _ => Spec_Axioms [specAxiom "gt1" (n > 1)])).
+       Spec_Cons "n" (def T T__pf) Pred_Trivial
+                   (fun n _ =>
+                      Spec_Cons "gt1" (n>1) Pred_Trivial
+                                (fun _ _ => Spec_Nil))).
 
 (* Example 4: Monoids *)
 Definition spec_example_monoid :=
-  Spec_ConsOp
+  Spec_Cons
     "T" Set Pred_Trivial
     (fun T _ =>
-       Spec_ConsOp
+       Spec_Cons
          "m_zero" T Pred_Trivial
          (fun m_zero _ =>
-            Spec_ConsOp
+            Spec_Cons
               "m_plus" (T -> T -> T) Pred_Trivial
               (fun m_plus _ =>
-                 Spec_Axioms
-                   [specAxiom "m_zero_left" (forall x, m_plus m_zero x = x);
-                     specAxiom "m_zero_right" (forall x, m_plus x m_zero = x);
-                     specAxiom "m_plus_assoc"
+                 Spec_Cons
+                   "m_zero_left" (forall x, m_plus m_zero x = x) Pred_Trivial
+                   (fun _ _ =>
+                      Spec_Cons
+                        "m_zero_right" (forall x, m_plus x m_zero = x) Pred_Trivial
+                        (fun _ _ =>
+                           Spec_Cons
+                             "m_plus_assoc"
                              (forall x y z,
-                                m_plus x (m_plus y z) = m_plus (m_plus x y) z)]))).
+                                m_plus x (m_plus y z) = m_plus (m_plus x y) z)
+                             Pred_Trivial
+                             (fun _ _ => Spec_Nil)))))).
 
 (* Example 5: Groups *)
 Definition spec_example_group :=
-  Spec_ConsOp
+  Spec_Cons
     "T" Set Pred_Trivial
     (fun T _ =>
-       Spec_ConsOp
+       Spec_Cons
          "g_zero" T Pred_Trivial
          (fun g_zero _ =>
-            Spec_ConsOp
+            Spec_Cons
               "g_plus" (T -> T -> T) Pred_Trivial
               (fun g_plus _ =>
-                 Spec_ConsOp
+                 Spec_Cons
                    "g_inv" (T -> T) Pred_Trivial
                    (fun g_inv _ =>
-                        Spec_Axioms
-                          [specAxiom "g_zero_left" (forall x, g_plus g_zero x = x);
-                            specAxiom "g_zero_right" (forall x, g_plus x g_zero = x);
-                            specAxiom "g_plus_assoc"
-                                    (forall x y z,
-                                       g_plus x (g_plus y z) = g_plus (g_plus x y) z);
-                            specAxiom "g_inv_left"
-                                    (forall (x:T), g_plus (g_inv x) x = g_zero);
-                            specAxiom "g_inv_right"
-                                    (forall (x:T), g_plus x (g_inv x) = g_zero)
-    ])))).
+                      Spec_Cons
+                        "g_zero_left" (forall x, g_plus g_zero x = x) Pred_Trivial
+                        (fun _ _ =>
+                           Spec_Cons
+                             "g_zero_right" (forall x, g_plus x g_zero = x) Pred_Trivial
+                             (fun _ _ =>
+                                Spec_Cons
+                                  "g_plus_assoc"
+                                  (forall x y z,
+                                     g_plus x (g_plus y z) = g_plus (g_plus x y) z)
+                                  Pred_Trivial
+                                  (fun _ _ =>
+                                     Spec_Cons
+                                       "g_inv_left"
+                                       (forall (x:T), g_plus (g_inv x) x = g_zero)
+                                       Pred_Trivial
+                                       (fun _ _ =>
+                                          Spec_Cons
+                                            "g_inv_right"
+                                            (forall (x:T), g_plus x (g_inv x) = g_zero)
+                                            Pred_Trivial
+                                            (fun _ _ => Spec_Nil))))))))).
 
 (* Example 6: The Natural Numbers as a Monoid *)
 Definition spec_example_natmonoid :=
-Spec_ConsOp "T" Type (@Pred_Eq Type nat)
+Spec_Cons "T" Type (@Pred_Eq Type nat)
   (fun T__param T__proof =>
-   Spec_ConsOp "m_zero" (def T__param T__proof) (Pred_Eq 0)
+   Spec_Cons "m_zero" (def T__param T__proof) (Pred_Eq 0)
      (fun m_zero__param m_zero__proof =>
-      Spec_ConsOp "m_plus"
+      Spec_Cons "m_plus"
         (def T__param T__proof ->
          def T__param T__proof -> def T__param T__proof) 
         (Pred_Eq Nat.add)
         (fun m_plus__param m_plus__proof
          =>
-         Spec_Axioms
-           (specAxiom "m_zero_left"
-              (forall x : def T__param T__proof,
-               def m_plus__param m_plus__proof
-                 (def m_zero__param m_zero__proof) x = x)
-            :: (specAxiom "m_zero_right"
+           Spec_Cons
+             "m_zero_left"
+             (forall x : def T__param T__proof,
+                def m_plus__param m_plus__proof
+                    (def m_zero__param m_zero__proof) x = x)
+             Pred_Trivial
+             (fun _ _ =>
+                Spec_Cons
+                  "m_zero_right"
                   (forall x : def T__param T__proof,
-                   def m_plus__param m_plus__proof x
-                     (def m_zero__param m_zero__proof) = x)
-                :: specAxiom "m_plus_assoc"
-                     (forall x y z : def T__param T__proof,
-                      def m_plus__param m_plus__proof x
-                        (def m_plus__param m_plus__proof y z) =
-                      def m_plus__param m_plus__proof
-                        (def m_plus__param m_plus__proof x y) z) :: nil)%list)))).
+                     def m_plus__param m_plus__proof x
+                         (def m_zero__param m_zero__proof) = x)
+                  Pred_Trivial
+                  (fun _ _ =>
+                     Spec_Cons
+                       "m_plus_assoc"
+                       (forall x y z : def T__param T__proof,
+                          def m_plus__param m_plus__proof x
+                              (def m_plus__param m_plus__proof y z) =
+                          def m_plus__param m_plus__proof
+                              (def m_plus__param m_plus__proof x y) z)
+                       Pred_Trivial
+                       (fun _ _ => Spec_Nil)))))).
 
-Definition spec_example_ops_natmonoid
+(*
+Definition spec_example_model_natmonoid
            T__param T__proof m_zero__param m_zero__proof m_plus__param m_plus__proof :
-  spec_ops spec_example_natmonoid :=
+  spec_model spec_example_natmonoid :=
   (@existT) _ _ T__param
     ((@existT) _ _ T__proof
        ((@existT) _ _ m_zero__param
           ((@existT) _ _ m_zero__proof
              ((@existT) _ _ m_plus__param
                 ((@existT) _ _ m_plus__proof ((@tt))))))).
+*)
 
 Definition spec_example_model_natmonoid
            T__param T__proof m_zero__param m_zero__proof m_plus__param m_plus__proof
@@ -305,115 +301,80 @@ Definition spec_example_model_natmonoid
                     (def m_plus__param m_plus__proof y z) =
                 def m_plus__param m_plus__proof
                     (def m_plus__param m_plus__proof x y) z) :
-  spec_model spec_example_natmonoid
-             (spec_example_ops_natmonoid T__param T__proof m_zero__param
-                                         m_zero__proof m_plus__param m_plus__proof) :=
-  conj m_zero_left__param (conj m_zero_right__param m_plus_assoc__param).
+  spec_model spec_example_natmonoid :=
+  @modelCons
+    _ (Pred_Eq (nat:Type)) _ T__param T__proof
+    (@modelCons
+       _ (Pred_Eq 0) _ m_zero__param m_zero__proof
+       (@modelCons
+          _ (Pred_Eq plus) _ m_plus__param m_plus__proof
+          (@modelCons
+             _ Pred_Trivial _ m_zero_left__param I
+             (@modelCons
+                _ Pred_Trivial _ m_zero_right__param I
+                (@modelCons
+                   _ Pred_Trivial _ m_plus_assoc__param I
+                   tt))))).
 
 
 (*** Interpretations ***)
 
-(* An interpretation from spec1 into spec2 is a pair of functions that map the
-ops and the models, respectively, of spec2 to those of spec1 *)
-Definition Interpretation spec1 spec2 :=
-  { ops_f: spec_ops spec2 -> spec_ops spec1 |
-    forall ops, spec_model spec2 ops -> spec_model spec1 (ops_f ops) }.
-
-(* Helper to build an interpretation from spec1 to spec2 *)
-Definition mkInterp {spec1 spec2} ops_f model_f : Interpretation spec1 spec2 :=
-  exist _ ops_f model_f.
-
-(* Apply the ops map of an interpretation *)
-Definition map_ops {spec1 spec2} (i:Interpretation spec1 spec2) :
-  spec_ops spec2 -> spec_ops spec1 :=
-  match i with exist _ ops_f model_f => ops_f end.
-
-(* Apply the model map of an interpretation *)
-Definition map_model {spec1 spec2} (i:Interpretation spec1 spec2) :
-  forall ops2, spec_model spec2 ops2 -> spec_model spec1 (map_ops i ops2) :=
-  match i with exist _ ops_f model_f => model_f end.
+(* An interpretation from spec1 into spec2 is a function from models of spec2 to
+models of spec1 *)
+Definition Interpretation spec1 spec2 := spec_model spec2 -> spec_model spec1.
 
 (* The identity interpretation *)
-Definition interp_id (spec:Spec) : Interpretation spec spec :=
-  mkInterp id (fun _ model => model).
+Definition interp_id (spec:Spec) : Interpretation spec spec := id.
 
 (* Composing interpretations *)
 Definition interp_compose {s1 s2 s3}
            (i2: Interpretation s2 s3) (i1: Interpretation s1 s2) :
   Interpretation s1 s3 :=
-  mkInterp (fun ops3 => map_ops i1 (map_ops i2 ops3))
-           (fun ops3 model3 => map_model i1 _ (map_model i2 _ model3)).
+  (fun model3 => i1 (i2 model3)).
 
 (* Build an interpretation between the tails of two specs that have the same
 head into an interpretation between the whole of the two specs *)
 Definition interp_cons f T (oppred: OpPred T)
            {spec1 spec2 : forall t, oppred t -> Spec}
            (i: forall t pfs, Interpretation (spec1 t pfs) (spec2 t pfs)) :
-  Interpretation (Spec_ConsOp f T oppred spec1)
-                 (Spec_ConsOp f T oppred spec2) :=
-  mkInterp (fun ops2:spec_ops (Spec_ConsOp f T oppred spec2) =>
-              let (t_o,o) := ops2 in
-              let (pf_o, rest_o) := o in
-              ops_cons t_o pf_o (map_ops (i _ _) rest_o))
-           (fun ops2 =>
-              match ops2
-                    return spec_model (Spec_ConsOp f T oppred spec2) ops2 ->
-                           spec_model
-                             (Spec_ConsOp f T oppred spec1)
-                             (let (t_o,o) := ops2 in
-                              let (pf_o,rest_o) := o in
-                              ops_cons t_o pf_o (map_ops (i _ _) rest_o)) with
-                | existT _ t_o (existT _ pf_o rest_o) =>
-                  fun model2 =>
-                    map_model (i t_o pf_o) rest_o model2
-              end).
+  Interpretation (Spec_Cons f T oppred spec1)
+                 (Spec_Cons f T oppred spec2) :=
+  (fun model2:spec_model (Spec_Cons f T oppred spec2) =>
+     let (t_o,pf_o,rest_o) := model2 in
+     modelCons t_o pf_o (i _ _ rest_o)).
 
 (* The simpler version, that does not destruct ops2. We choose the above version
 to make it more efficient to compute with this interpretation. *)
 (*
-Definition interp_cons f T (oppred: OpPred T)
+Definition interp_cons2 f T (oppred: OpPred T)
            {spec1 spec2 : forall t, oppred t -> Spec}
            (i: forall t pfs, Interpretation (spec1 t pfs) (spec2 t pfs)) :
-  Interpretation (Spec_ConsOp f T oppred spec1)
-                 (Spec_ConsOp f T oppred spec2) :=
-  mkInterp (fun ops2 =>
-              ops_cons (ops_head ops2) (ops_proof ops2)
-                       (map_ops (i _ _) (ops_rest ops2)))
-           (fun ops2 model2 =>
-              map_model (i _ _) _ model2).
+  Interpretation (Spec_Cons f T oppred spec1)
+                 (Spec_Cons f T oppred spec2) :=
+  (fun model2 =>
+     modelCons (model_head model2) (model_proof model2)
+                (i _ _ (model_rest model2))).
 *)
 
 (* Take an interpretation from spec1 to spec2 and cons an op onto spec2 *)
 Definition interp_cons_r f T (oppred: OpPred T)
            {spec1} {spec2: forall t, oppred t -> Spec}
            (i: forall t pfs, Interpretation spec1 (spec2 t pfs)) :
-  Interpretation spec1 (Spec_ConsOp f T oppred spec2) :=
-  mkInterp (fun ops2:spec_ops (Spec_ConsOp f T oppred spec2) =>
-              let (t_o,o) := ops2 in
-              let (pf_o,rest_o) := o in
-              map_ops (i t_o pf_o) rest_o)
-           (fun ops2 =>
-              match ops2
-                    return spec_model (Spec_ConsOp f T oppred spec2) ops2 ->
-                           spec_model spec1
-                                      (let (t_o,o) := ops2 in
-                                       let (pf_o,rest_o) := o in
-                                       map_ops (i _ _) rest_o) with
-                | existT _ t_o (existT _ pf_o rest_o) =>
-                  fun model2 =>
-                    map_model (i t_o pf_o) rest_o model2
-              end).
+  Interpretation spec1 (Spec_Cons f T oppred spec2) :=
+  (fun model2:spec_model (Spec_Cons f T oppred spec2) =>
+     let (t_o,pf_o,rest_o) := model2 in
+     i t_o pf_o rest_o).
 
 
 (* The simpler version, that does not destruct ops2. We choose the above version
 to make it more efficient to compute with this interpretation. *)
 (*
-Definition interp_cons_r f T (oppred: OpPred T)
+Definition interp_cons_r2 f T (oppred: OpPred T)
            {spec1} {spec2: forall t, oppred t -> Spec}
            (i: forall t pfs, Interpretation spec1 (spec2 t pfs)) :
-  Interpretation spec1 (Spec_ConsOp f T oppred spec2) :=
-  mkInterp (fun ops2 => map_ops (i (ops_head ops2) (ops_proof ops2)) (ops_rest ops2))
-           (fun ops2 model2 => map_model (i (ops_head ops2) (ops_proof ops2)) _ model2).
+  Interpretation spec1 (Spec_Cons f T oppred spec2) :=
+  (fun model2 =>
+    i (model_head model2) (model_proof model2) (model_rest model2)).
 *)
 
 
@@ -421,19 +382,28 @@ Definition interp_cons_r f T (oppred: OpPred T)
 
 (* Interpret T as nat and n as n for spec_example_3 into spec_example_2 *)
 Program Definition interp_example_3_2 : Interpretation spec_example_3 spec_example_2 :=
-  fun ops2 =>
-    (ops_cons (oppred:= Pred_Eq nat) nat eq_refl
-              (ops_cons (oppred:=Pred_Trivial) (ops_head ops2) I (tt : spec_ops (Spec_Axioms _)))) : spec_ops spec_example_3.
+  fun model2 =>
+    match model2 with
+      | modelCons n n__proof tt =>
+        (modelCons
+           (oppred:=Pred_Eq nat) nat eq_refl
+           (modelCons (oppred:=Pred_Trivial) n _
+                      (modelCons
+                         (oppred:=Pred_Trivial)
+                         _ _
+                         (tt: spec_model Spec_Nil))))
+    end.
 
 
 (*** Appending Specs ***)
 
+(*
 (* Append axioms to the end of a spec *)
 Fixpoint spec_append_axioms spec axioms2 : Spec :=
   match spec with
     | Spec_Axioms axioms1 => Spec_Axioms (axioms1 ++ axioms2)
-    | Spec_ConsOp f T oppred rest =>
-      Spec_ConsOp f T oppred (fun t pf => spec_append_axioms (rest t pf) axioms2)
+    | Spec_Cons f T oppred rest =>
+      Spec_Cons f T oppred (fun t pf => spec_append_axioms (rest t pf) axioms2)
   end.
 
 Lemma conjoin_axioms_append1 axioms1 axioms2 :
@@ -460,7 +430,7 @@ Fixpoint append_axioms_interp1 spec axioms2 :
       mkInterp 
         (spec1:=Spec_Axioms axioms1) (spec2:=Spec_Axioms (axioms1++axioms2))
         id (fun _ model => conjoin_axioms_append1 axioms1 axioms2 model)
-    | Spec_ConsOp f T oppred rest =>
+    | Spec_Cons f T oppred rest =>
       interp_cons f T oppred (fun t pf => append_axioms_interp1 (rest t pf) axioms2)
   end.
 
@@ -473,25 +443,27 @@ Fixpoint append_axioms_interp2 spec axioms2 :
         (spec1:=Spec_Axioms axioms2) (spec2:=Spec_Axioms (axioms1++axioms2))
         (fun _ => tt)
         (fun _ model => conjoin_axioms_append2 axioms1 axioms2 model)
-    | Spec_ConsOp f T oppred rest =>
+    | Spec_Cons f T oppred rest =>
       interp_cons_r f T oppred
                     (fun t pf => append_axioms_interp2 (rest t pf) axioms2)
   end.
+*)
 
 (* Append one spec after another, where the spec being appended can depend on
-the ops of the spec it is coming after *)
-Fixpoint spec_append spec1 : (spec_ops spec1 -> Spec) -> Spec :=
-  match spec1 return (spec_ops spec1 -> Spec) -> Spec with
-    | Spec_Axioms axioms1 =>
-      fun spec2 => spec_append_axioms (spec2 tt) axioms1
-    | Spec_ConsOp f T oppred rest =>
+the model of the spec it is coming after *)
+Fixpoint spec_append spec1 : (spec_model spec1 -> Spec) -> Spec :=
+  match spec1 return (spec_model spec1 -> Spec) -> Spec with
+    | Spec_Nil => 
+      fun spec2 => spec2 tt
+    | Spec_Cons f T oppred rest =>
       fun spec2 =>
-        Spec_ConsOp f T oppred
+        Spec_Cons f T oppred
                     (fun t pf =>
                        spec_append (rest t pf)
-                                   (fun ops1 => spec2 (ops_cons t pf ops1)))
+                                   (fun model1 => spec2 (modelCons t pf model1)))
   end.
 
+(*
 (* Helper for the next definition *)
 Definition append_axioms_interp spec spec1 axioms2
            (ops_f : spec_ops spec1 -> spec_ops spec)
@@ -506,190 +478,102 @@ Definition append_axioms_interp spec spec1 axioms2
               model_f (map_ops (append_axioms_interp1 spec1 axioms2) ops1)
                       (map_model (append_axioms_interp2 spec1 axioms2) ops1 model1)
                       (map_model (append_axioms_interp1 spec1 axioms2) ops1 model1)).
+*)
 
 (* The interpretation from a spec to the result of appending another spec to it *)
 Fixpoint interp_append1 spec1 :
   forall spec2, Interpretation spec1 (spec_append spec1 spec2) :=
   match spec1 return
         forall spec2, Interpretation spec1 (spec_append spec1 spec2) with
-    | Spec_Axioms axioms1 =>
-      fun spec2 => append_axioms_interp2 (spec2 tt) axioms1
-    | Spec_ConsOp f T oppred rest =>
+    | Spec_Nil =>
+      fun spec2 => (fun _ => tt)
+    | Spec_Cons f T oppred rest =>
       fun spec2 =>
         interp_cons f T oppred
                     (fun t pf =>
                        interp_append1 (rest t pf)
-                                      (fun ops1 => spec2 (ops_cons t pf ops1)))
+                                      (fun model1 => spec2 (modelCons t pf model1)))
   end.
 
-(* Extract the ops for spec2 from ops for (spec_append spec1 spec2). This
-function, along with interp_append2_model, below, is essentially a dependent
-interpretation, i.e., an Interpretation spec2 (spec_append spec1 spec2) where
-spec2 depends on the ops being passed in for (spec_append spec1 spec2). *)
-Fixpoint interp_append2_ops spec1 :
-  forall spec2 (ops12: spec_ops (spec_append spec1 spec2)),
-    spec_ops (spec2 (map_ops (interp_append1 spec1 spec2) ops12)) :=
+(* Extract the model for spec2 from the model for (spec_append spec1 spec2).
+This function, along with interp_append2_model, below, is essentially a
+dependent interpretation, i.e., an Interpretation spec2 (spec_append spec1
+spec2) where spec2 depends on the model of (spec_append spec1 spec2). *)
+Fixpoint interp_append2_model spec1 :
+  forall spec2 (model12: spec_model (spec_append spec1 spec2)),
+    spec_model (spec2 (interp_append1 spec1 spec2 model12)) :=
   match spec1 with
-    | Spec_Axioms axioms1 =>
-      fun spec2 ops12 =>
-        match (map_ops (interp_append1 (Spec_Axioms axioms1) spec2) ops12) as ops1
-              return spec_ops (spec2 ops1) with
-          | tt => map_ops (append_axioms_interp1 _ _) ops12
+    | Spec_Nil =>
+      fun spec2 model12 =>
+        match (interp_append1 Spec_Nil spec2 model12) as model1
+              return spec_model (spec2 model1) with
+          | tt => model12
         end
-    | Spec_ConsOp f T oppred rest =>
-      fun spec2 ops12 =>
-        match ops12 return
-              spec_ops (spec2 (map_ops (interp_append1 _ spec2) ops12)) with
-          | existT _ t (existT _ pf ops12') =>
-            interp_append2_ops (rest t pf) (fun ops1 => spec2 (ops_cons t pf ops1))
-                               ops12'
+    | Spec_Cons f T oppred rest =>
+      fun spec2 model12 =>
+        match model12 return
+              spec_model (spec2 (interp_append1 _ spec2 model12)) with
+          | modelCons t pf model12' =>
+            interp_append2_model
+              (rest t pf) (fun model1 => spec2 (modelCons t pf model1))
+              model12'
         end
   end.
-
-(* Extract a model of spec2 from a model of (spec_append spec1 spec2). This is
-like a dependent interpretation; see the comments for interp2_append2_ops. *)
-Lemma interp_append2_model spec1 spec2
-      (ops12: spec_ops (spec_append spec1 spec2))
-      (model12: spec_model (spec_append spec1 spec2) ops12) :
-  spec_model (spec2 (map_ops (interp_append1 spec1 spec2) ops12))
-             (interp_append2_ops spec1 spec2 ops12).
-  revert spec2 ops12 model12; induction spec1; intros.
-  unfold interp_append2_ops.
-  destruct (map_ops (interp_append1 (Spec_Axioms axioms) spec2) ops12).
-  apply map_model; apply model12.
-  destruct ops12 as [ t x ]; destruct x as [ pf ops12' ].
-  apply (H t pf (fun ops1 : spec_ops (rest t pf) => spec2 (ops_cons t pf ops1))).
-  assumption.
-Qed.
 
 (* Build an interpretation into the append of two specs from a funky binary sort
 of interpretation into the two specs that are being appended. *)
 Definition interp_append spec spec1 spec2
-           (ops_f: forall ops1, spec_ops (spec2 ops1) -> spec_ops spec)
-           (model_f:
-              forall ops1 ops2,
-                spec_model spec1 ops1 -> spec_model (spec2 ops1) ops2 ->
-                spec_model spec (ops_f ops1 ops2)) :
+           (i: forall model1, spec_model (spec2 model1) -> spec_model spec) :
   Interpretation spec (spec_append spec1 spec2) :=
-  mkInterp
-    (fun ops12 =>
-       ops_f (map_ops (interp_append1 spec1 spec2) ops12)
-             (interp_append2_ops spec1 spec2 ops12))
-    (fun ops12 model12 =>
-       model_f (map_ops (interp_append1 spec1 spec2) ops12)
-               (interp_append2_ops spec1 spec2 ops12)
-               (map_model (interp_append1 spec1 spec2) ops12 model12)
-               (interp_append2_model spec1 spec2 ops12 model12)).
+  fun model12 =>
+       i (interp_append1 spec1 spec2 model12)
+         (interp_append2_model spec1 spec2 model12).
 
 
 (*** Spec Overlap ***)
 
 (* NotInSpec f spec is a proof that f is not used as an op name in spec *)
 Inductive NotInSpec (f:Field) : Spec -> Prop :=
-| NotInSpec_base axioms : NotInSpec f (Spec_Axioms axioms)
+| NotInSpec_nil : NotInSpec f Spec_Nil
 | NotInSpec_cons f' T oppred rest :
     f <> f' ->
     (forall t pf, NotInSpec f (rest t pf)) ->
-    NotInSpec f (Spec_ConsOp f' T oppred rest)
+    NotInSpec f (Spec_Cons f' T oppred rest)
 .
 
 (* Tactic to prove NotInSpec goals *)
 Ltac prove_not_in_spec :=
   match goal with
-    | |- NotInSpec ?f (Spec_ConsOp ?f' _ _ _) =>
+    | |- NotInSpec ?f (Spec_Cons ?f' _ _ _) =>
       apply NotInSpec_cons; [ discriminate | intros; prove_not_in_spec ]
-    | |- NotInSpec ?f (Spec_Axioms _) =>
-      apply NotInSpec_base
+    | |- NotInSpec ?f Spec_Nil =>
+      apply NotInSpec_nil
   end.
-
-(* Helper lemma to prove not in goals *)
-Lemma not_in_cons {A} (x y:A) l :
-  y <> x -> ~(In x l) -> ~(In x (y::l)).
-  intros neq not_in in_xy.
-  destruct in_xy; contradiction.
-Qed.
-
-(* Tactic to prove ~(In f l) goals *)
-Ltac prove_not_in_list :=
-  match goal with
-    | |- ~(In ?f (cons ?f' ?l)) =>
-      apply not_in_cons; [ discriminate | prove_not_in_list ]
-    | |- ~(In ?f nil) =>
-      apply in_nil
-  end.
-
-(* Helper type for SpecOverlap *)
-Inductive AxiomOverlap : list SpecAxiom -> list SpecAxiom -> Type :=
-| AxiomOverlap_base : AxiomOverlap [] []
-| AxiomOverlap_eq ax_name ax_tp axioms1 axioms2 :
-    AxiomOverlap axioms1 axioms2 ->
-    AxiomOverlap (specAxiom ax_name ax_tp::axioms1)
-                 (specAxiom ax_name ax_tp::axioms2)
-| AxiomOverlap_neq1 ax_name ax_tp axioms1 axioms2 :
-    ~(In ax_name (map axiom_name axioms2)) ->
-    AxiomOverlap axioms1 axioms2 ->
-    AxiomOverlap (specAxiom ax_name ax_tp::axioms1) axioms2
-| AxiomOverlap_neq2 ax_name ax_tp axioms1 axioms2 :
-    ~(In ax_name (map axiom_name axioms1)) ->
-    AxiomOverlap axioms1 axioms2 ->
-    AxiomOverlap axioms1 (specAxiom ax_name ax_tp::axioms2)
-.
 
 (* SpecOverlap spec1 spec2 is a correlation between spec1 and spec2 that
 identifies some sequence of ops and axioms that occur in both spec1 and spec2 in
 the same order and with the same types and subtype predictes. In fact, an
 element of SpecOverlap spec1 spec2 is the maximal such sequence. *)
 Inductive SpecOverlap : Spec -> Spec -> Type :=
-| SpecOverlap_base axioms1 axioms2 :
-    AxiomOverlap axioms1 axioms2 ->
-    SpecOverlap (Spec_Axioms axioms1) (Spec_Axioms axioms2)
+| SpecOverlap_nil : SpecOverlap Spec_Nil Spec_Nil
 | SpecOverlap_eq f T oppred rest1 rest2 :
     (forall t pf, SpecOverlap (rest1 t pf) (rest2 t pf)) ->
-    SpecOverlap (Spec_ConsOp f T oppred rest1) (Spec_ConsOp f T oppred rest2)
+    SpecOverlap (Spec_Cons f T oppred rest1) (Spec_Cons f T oppred rest2)
 | SpecOverlap_neq1 f1 T1 oppred1 rest1 spec2 :
     NotInSpec f1 spec2 ->
     (forall t pf, SpecOverlap (rest1 t pf) spec2) ->
-    SpecOverlap (Spec_ConsOp f1 T1 oppred1 rest1) spec2
+    SpecOverlap (Spec_Cons f1 T1 oppred1 rest1) spec2
 | SpecOverlap_neq2 f2 T2 oppred2 rest2 spec1 :
     NotInSpec f2 spec1 ->
     (forall t pf, SpecOverlap spec1 (rest2 t pf)) ->
-    SpecOverlap spec1 (Spec_ConsOp f2 T2 oppred2 rest2)
+    SpecOverlap spec1 (Spec_Cons f2 T2 oppred2 rest2)
 .
-
-(* Tactic to prove AxiomOverlap *)
-Ltac prove_axiom_overlap :=
-  lazymatch goal with
-    | |- AxiomOverlap (specAxiom ?ax_name1 ?ax_tp1 :: ?axioms1)
-                      (specAxiom ?ax_name2 ?ax_tp2 :: ?axioms2) =>
-      match eval hnf in (Field_dec ax_name1 ax_name2) with
-        | left _ =>
-          (apply AxiomOverlap_eq
-                 || fail "Non-matching types at axiom" ax_name1);
-          intros; prove_axiom_overlap
-        | right ?neq =>
-          ((apply AxiomOverlap_neq1; [ prove_not_in_list | ]) ||
-           (apply AxiomOverlap_neq2; [ prove_not_in_list | ]) ||
-           fail "The axioms " ax_name1 " and " ax_name2 " appear to be in a different order in the two axioms");
-          prove_axiom_overlap
-      end
-    | |- AxiomOverlap (cons _ _) nil =>
-      apply AxiomOverlap_neq1; [ apply in_nil | prove_axiom_overlap ]
-    | |- AxiomOverlap nil (cons _ _) =>
-      apply AxiomOverlap_neq2; [ apply in_nil | prove_axiom_overlap ]
-    | |- AxiomOverlap nil nil =>
-      apply AxiomOverlap_base
-    | |- AxiomOverlap ?axioms1 ?axioms2 =>
-      let axioms1_hnf := (eval hnf in axioms1) in
-      let axioms2_hnf := (eval hnf in axioms2) in
-      progress (change (AxiomOverlap axioms1_hnf axioms2_hnf)); prove_axiom_overlap
-    | |- ?goal => fail "prove_axiom_overlap: not an AxiomOverlap goal: " goal
-  end.
 
 (* Tactic to prove spec overlap *)
 Ltac prove_spec_overlap :=
   lazymatch goal with
-    | |- SpecOverlap (Spec_ConsOp ?f1 ?T1 ?oppred1 ?rest1)
-                     (Spec_ConsOp ?f2 ?T2 ?oppred2 ?rest2) =>
+    | |- SpecOverlap (Spec_Cons ?f1 ?T1 ?oppred1 ?rest1)
+                     (Spec_Cons ?f2 ?T2 ?oppred2 ?rest2) =>
       lazymatch eval hnf in (Field_dec f1 f2) with
         | left _ =>
           (apply SpecOverlap_eq
@@ -703,12 +587,12 @@ Ltac prove_spec_overlap :=
            fail "The fields " f1 " and " f2 " appear to be in a different order in the two specs");
           prove_spec_overlap
       end
-    | |- SpecOverlap (Spec_ConsOp _ _ _ _) (Spec_Axioms _) =>
-      apply SpecOverlap_neq1; [ apply NotInSpec_base | intros; prove_spec_overlap ]
-    | |- SpecOverlap (Spec_Axioms _) (Spec_ConsOp _ _ _ _) =>
-      apply SpecOverlap_neq2; [ apply NotInSpec_base | intros; prove_spec_overlap ]
-    | |- SpecOverlap (Spec_Axioms _) (Spec_Axioms _) =>
-      apply SpecOverlap_base; prove_axiom_overlap
+    | |- SpecOverlap (Spec_Cons _ _ _ _) Spec_Nil =>
+      apply SpecOverlap_neq1; [ apply NotInSpec_nil | intros; prove_spec_overlap ]
+    | |- SpecOverlap Spec_Nil (Spec_Cons _ _ _ _) =>
+      apply SpecOverlap_neq2; [ apply NotInSpec_nil | intros; prove_spec_overlap ]
+    | |- SpecOverlap Spec_Nil Spec_Nil =>
+      apply SpecOverlap_nil
     | |- SpecOverlap ?spec1 ?spec2 =>
       let spec1_hnf := (eval hnf in spec1) in
       let spec2_hnf := (eval hnf in spec2) in
@@ -722,8 +606,8 @@ Ltac prove_spec_overlapN n :=
     | 0 => idtac "prove_spec_overlapN: n exhausted"
     | S ?n' =>
       lazymatch goal with
-        | |- SpecOverlap (Spec_ConsOp ?f1 ?T1 ?oppred1 ?rest1)
-                         (Spec_ConsOp ?f2 ?T2 ?oppred2 ?rest2) =>
+        | |- SpecOverlap (Spec_Cons ?f1 ?T1 ?oppred1 ?rest1)
+                         (Spec_Cons ?f2 ?T2 ?oppred2 ?rest2) =>
           idtac "prove_spec_overlapN: cons-cons";
           lazymatch eval hnf in (Field_dec f1 f2) with
             | left _ =>
@@ -738,15 +622,15 @@ Ltac prove_spec_overlapN n :=
                fail "The fields " f1 " and " f2 " appear to be in a different order in the two specs");
               prove_spec_overlapN n'
           end
-        | |- SpecOverlap (Spec_ConsOp _ _ _ _) (Spec_Axioms _) =>
+        | |- SpecOverlap (Spec_Cons _ _ _ _) Spec_Nil =>
           idtac "prove_spec_overlapN: cons-axiom";
-          apply SpecOverlap_neq1; [ apply NotInSpec_base | intros; prove_spec_overlapN n' ]
-        | |- SpecOverlap (Spec_Axioms _) (Spec_ConsOp _ _ _ _) =>
+          apply SpecOverlap_neq1; [ apply NotInSpec_nil | intros; prove_spec_overlapN n' ]
+        | |- SpecOverlap Spec_Nil (Spec_Cons _ _ _ _) =>
           idtac "prove_spec_overlapN: axiom-cons";
-          apply SpecOverlap_neq2; [ apply NotInSpec_base | intros; prove_spec_overlapN n' ]
-        | |- SpecOverlap (Spec_Axioms _) (Spec_Axioms _) =>
+          apply SpecOverlap_neq2; [ apply NotInSpec_nil | intros; prove_spec_overlapN n' ]
+        | |- SpecOverlap Spec_Nil Spec_Nil =>
           idtac "prove_spec_overlapN: axiom-axiom";
-          apply SpecOverlap_base; prove_axiom_overlap
+          apply SpecOverlap_nil
         | |- SpecOverlap ?spec1 ?spec2 =>
           idtac "prove_spec_overlapN: hnf";
           let spec1_hnf := (eval hnf in spec1) in
@@ -759,137 +643,83 @@ Ltac prove_spec_overlapN n :=
 
 (*** Spec Substitution ***)
 
-(* Helper for spec_subtract: return all axioms in the axioms1 list that do not
-overlap with the axioms in axioms2 *)
-Fixpoint axioms_subtract axioms1 axioms2
-         (overlap: AxiomOverlap axioms1 axioms2) : list SpecAxiom :=
-  match overlap with
-    | AxiomOverlap_base => []
-    | AxiomOverlap_eq ax_name ax_tp axioms1 axioms2 overlap' =>
-      axioms_subtract axioms1 axioms2 overlap'
-    | AxiomOverlap_neq1 ax_name ax_tp axioms1' axioms2' not_in overlap' =>
-      (specAxiom ax_name ax_tp)
-        :: axioms_subtract axioms1' axioms2' overlap'
-    | AxiomOverlap_neq2 ax_name ax_tp axioms1' axioms2' not_in overlap' =>
-      axioms_subtract axioms1' axioms2' overlap'
-  end.
-
-(* If you subtract axioms2 from axioms1 and then add them back again you can
-prove the original axioms1. *)
-Lemma axioms_subtract_interp axioms1 axioms2 overlap :
-  conjoin_axioms axioms2 ->
-  conjoin_axioms (axioms_subtract axioms1 axioms2 overlap) ->
-  conjoin_axioms axioms1.
-  induction overlap; intros.
-  trivial.
-  destruct (conjoin_axioms_destruct _ _ _ H).
-  apply conjoin_axioms_cons; [ assumption | apply IHoverlap; assumption ].
-  destruct (conjoin_axioms_destruct _ _ _ H0).
-  apply conjoin_axioms_cons; [ assumption | apply IHoverlap; assumption ].
-  destruct (conjoin_axioms_destruct _ _ _ H).
-  apply IHoverlap; assumption.
-Qed.
-
-(* Subtract the overlapping ops and axioms in spec2 from spec1. Note that this
-operation requires ops for spec2. *)
+(* Subtract the overlapping ops in spec2 from spec1. Note that this operation
+requires a model for spec2. *)
 Fixpoint spec_subtract spec1 spec2 (overlap: SpecOverlap spec1 spec2) :
-  spec_ops spec2 -> Spec :=
-  match overlap in SpecOverlap spec1 spec2 return spec_ops spec2 -> Spec with
-    | SpecOverlap_base axioms1 axioms2 overlap' =>
-      fun _ => Spec_Axioms (axioms_subtract axioms1 axioms2 overlap')
+  spec_model spec2 -> Spec :=
+  match overlap in SpecOverlap spec1 spec2 return spec_model spec2 -> Spec with
+    | SpecOverlap_nil =>
+      fun _ => Spec_Nil
     | SpecOverlap_eq f T oppred rest1 rest2 overlap' =>
-      fun ops2 =>
-        let (t,x) := ops2 in
-        let (pf,ops2') := x in
-        spec_subtract (rest1 t pf) (rest2 t pf) (overlap' t pf) ops2'
+      fun model2 =>
+        let (t,pf,model2') := model2 in
+        spec_subtract (rest1 t pf) (rest2 t pf) (overlap' t pf) model2'
     | SpecOverlap_neq1 f1 T1 oppred1 rest1 spec2 not_in overlap' =>
-      fun ops2 =>
-        Spec_ConsOp f1 T1 oppred1
+      fun model2 =>
+        Spec_Cons f1 T1 oppred1
                     (fun t pf =>
-                       spec_subtract (rest1 t pf) spec2 (overlap' t pf) ops2)
+                       spec_subtract (rest1 t pf) spec2 (overlap' t pf) model2)
     | SpecOverlap_neq2 f2 T2 oppred2 rest2 spec1 not_in overlap' =>
-      fun ops2 =>
-        let (t,x) := ops2 in
-        let (pf,ops2') := x in
-        spec_subtract spec1 (rest2 t pf) (overlap' t pf) ops2'
-  end.
-
-(* If you subtract spec2 from spec1 then you can recover all the ops of spec1 if
-you have ops for spec2 and for the subtraction. This definition, along with
-spec_subtract_interp_model, forms a binary sort of interpretation. *)
-Fixpoint spec_subtract_interp_ops spec1 spec2 (overlap : SpecOverlap spec1 spec2) :
-  forall (ops2:spec_ops spec2),
-  spec_ops (spec_subtract spec1 spec2 overlap ops2) ->
-  spec_ops spec1 :=
-  match overlap in SpecOverlap spec1 spec2
-        return forall ops2,
-                 spec_ops (spec_subtract spec1 spec2 overlap ops2) ->
-                 spec_ops spec1 with
-    | SpecOverlap_base axioms1 axioms2 overlap' =>
-      fun ops2 ops21 => tt
-    | SpecOverlap_eq f T oppred rest1 rest2 overlap' =>
-      fun ops2 =>
-        match ops2 return
-              spec_ops (spec_subtract
-                          _ _ (SpecOverlap_eq _ _ _ _ _ overlap') ops2) ->
-              spec_ops (Spec_ConsOp f T oppred rest1) with
-          | existT _ t (existT _ pf ops2') =>
-            fun ops21 =>
-              ops_cons t pf (spec_subtract_interp_ops _ _ (overlap' t pf) ops2' ops21)
-        end
-    | SpecOverlap_neq1 f1 T1 oppred1 rest1 spec2 not_in overlap' =>
-      fun ops2 ops21 =>
-        match ops21 return spec_ops (Spec_ConsOp f1 T1 oppred1 rest1) with
-          | existT _ t (existT _ pf ops21') =>
-            ops_cons t pf (spec_subtract_interp_ops _ _ (overlap' t pf) ops2 ops21')
-        end
-    | SpecOverlap_neq2 f2 T2 oppred2 rest2 spec1 not_in overlap' =>
-      fun ops2 =>
-        match ops2 return
-              spec_ops (spec_subtract
-                          _ _ (SpecOverlap_neq2 _ _ _ _ _ _ overlap') ops2) ->
-              spec_ops spec1 with
-          | existT _ t (existT _ pf ops2') =>
-            fun ops21 =>
-              spec_subtract_interp_ops _ _ (overlap' t pf) ops2' ops21
-        end
+      fun model2 =>
+        let (t,pf,model2') := model2 in
+        spec_subtract spec1 (rest2 t pf) (overlap' t pf) model2'
   end.
 
 (* If you subtract spec2 from spec1 then you can recover a model of spec1 if you
-have a model for spec2 and for the subtraction. This definition, along with
-spec_subtract_interp_ops, forms a binary sort of interpretation. *)
-Lemma spec_subtract_interp_model spec1 spec2 (overlap : SpecOverlap spec1 spec2) :
-  forall (ops2:spec_ops spec2) (model2:spec_model spec2 ops2)
-         (ops21:spec_ops (spec_subtract spec1 spec2 overlap ops2))
-         (model21:spec_model (spec_subtract spec1 spec2 overlap ops2) ops21),
-    spec_model spec1 (spec_subtract_interp_ops spec1 spec2 overlap ops2 ops21).
-  induction overlap; intros.
-  apply (axioms_subtract_interp axioms1 axioms2 a); assumption.
-  destruct ops2 as [t x]; destruct x as [pf ops2'].
-  apply H; assumption.
-  destruct ops21 as [t x]; destruct x as [pf ops21'].
-  apply H; assumption.
-  destruct ops2 as [t x]; destruct x as [pf ops2'].
-  apply H; assumption.
-Qed.
+have models for spec2 and for the subtraction. This definition forms a binary
+sort of interpretation of the pseudo-type (spec2, spec1 - spec2) -> spec1. *)
+Fixpoint spec_subtract_interp spec1 spec2 (overlap : SpecOverlap spec1 spec2) :
+  forall (model2:spec_model spec2),
+  spec_model (spec_subtract spec1 spec2 overlap model2) ->
+  spec_model spec1 :=
+  match overlap in SpecOverlap spec1 spec2
+        return forall model2,
+                 spec_model (spec_subtract spec1 spec2 overlap model2) ->
+                 spec_model spec1 with
+    | SpecOverlap_nil =>
+      fun model2 model21 => tt
+    | SpecOverlap_eq f T oppred rest1 rest2 overlap' =>
+      fun model2 =>
+        match model2 return
+              spec_model (spec_subtract
+                          _ _ (SpecOverlap_eq _ _ _ _ _ overlap') model2) ->
+              spec_model (Spec_Cons f T oppred rest1) with
+          | modelCons t pf model2' =>
+            fun model21 =>
+              modelCons t pf (spec_subtract_interp _ _ (overlap' t pf) model2' model21)
+        end
+    | SpecOverlap_neq1 f1 T1 oppred1 rest1 spec2 not_in overlap' =>
+      fun model2 model21 =>
+        match model21 return spec_model (Spec_Cons f1 T1 oppred1 rest1) with
+          | modelCons t pf model21' =>
+            modelCons t pf (spec_subtract_interp _ _ (overlap' t pf) model2 model21')
+        end
+    | SpecOverlap_neq2 f2 T2 oppred2 rest2 spec1 not_in overlap' =>
+      fun model2 =>
+        match model2 return
+              spec_model (spec_subtract
+                          _ _ (SpecOverlap_neq2 _ _ _ _ _ _ overlap') model2) ->
+              spec_model spec1 with
+          | modelCons t pf model2' =>
+            fun model21 =>
+              spec_subtract_interp _ _ (overlap' t pf) model2' model21
+        end
+  end.
 
 (* Build a spec using spec substitution *)
 Definition spec_subst {spec spec1 spec2}
            (overlap: SpecOverlap spec spec1) (i: Interpretation spec1 spec2) : Spec :=
   spec_append spec2
-              (fun ops2 =>
-                 spec_subtract spec spec1 overlap (map_ops i ops2)).
+              (fun model2 =>
+                 spec_subtract spec spec1 overlap (i model2)).
 
 (* Build the interpretation from spec1 to the result of applying spec
 substitution to spec1 *)
 Definition spec_subst_interp1 {spec spec1 spec2} overlap i :
-  Interpretation spec (@spec_subst spec spec1 spec2 overlap i).
-  unfold spec_subst.
-  eapply interp_append; intros.
-  apply spec_subtract_interp_model.
-  apply (map_model i _ H).
-  apply H0.
-Defined.
+  Interpretation spec (@spec_subst spec spec1 spec2 overlap i) :=
+  interp_append _ _ _
+                (fun model2 model_subtract =>
+                   spec_subtract_interp _ _ overlap (i model2) model_subtract).
 
 (* Build the interpretation from spec2 to the result of applying any spec
 substitution using an interpretation into spec2 *)
@@ -898,268 +728,11 @@ Definition spec_subst_interp2 {spec spec1 spec2} overlap i :
   interp_append1 _ _.
 
 
-(*** Quantifying over the Ops of a Spec ***)
+(*** Isomorphisms Between Specs and Types ***)
 
-Definition ForallOp T (oppred: OpPred T) : (forall t, oppred t -> Type) -> Type :=
-  match oppred return (forall t, sats_op_pred oppred t -> Type) -> Type with
-    | Pred_Trivial => fun A => forall t, A t I
-    | _ => fun A => forall t pf, A t pf
-  end.
-
-Definition LambdaOp T oppred : forall body_tp, (forall t pf, body_tp t pf) ->
-                                               ForallOp T oppred body_tp :=
-  match oppred return forall body_tp, (forall t pf, body_tp t pf) ->
-                                      ForallOp T oppred body_tp with
-    | Pred_Trivial => fun body_tp body => fun t => body t I
-    | _ => fun body_tp body => fun t pf => body t pf
-  end.
-
-Definition replace_op_proof T (oppred: OpPred T) : forall t, oppred t -> oppred t :=
-  match oppred return forall t, sats_op_pred oppred t ->
-                                sats_op_pred oppred t with
-    | Pred_Trivial => fun t _ => I
-    | _ => fun t pf => pf
-  end.
-
-(* Helper: all proofs of True are equal *)
-Definition True_eq (pf1: True) : forall pf2, pf1 = pf2 :=
-  match pf1 return forall pf2, pf1 = pf2 with
-    | I => fun pf2 => match pf2 return I = pf2 with I => eq_refl end end.
-
-(* Helper: all elements of unit are equal *)
-Definition unit_eq (u1: unit) : forall u2, u1 = u2 :=
-  match u1 return forall u2, u1 = u2 with
-    | tt => fun u2 => match u2 return tt = u2 with tt => eq_refl end end.
- 
-(* Replacing an op proof yields an equal proof (because a proof of True is a
-proof of True) *)
-Definition replace_op_proof_eq T (oppred: OpPred T) :
-  forall t pf, pf = replace_op_proof T oppred t pf :=
-  match oppred return forall t pf, pf = replace_op_proof T oppred t pf with
-    | Pred_Trivial => fun t _ => True_eq _ _
-    | _ => fun t pf => eq_refl
-  end.
-
-(* Apply an op function to an op and its proof *)
-Definition ApplyOp T (oppred: OpPred T) :
-  forall body_tp, ForallOp T oppred body_tp ->
-                  forall t pf, body_tp t (replace_op_proof T oppred t pf) :=
-  match oppred return forall body_tp,
-                        ForallOp T oppred body_tp ->
-                        forall t pf, body_tp t (replace_op_proof T oppred t pf) with
-    | Pred_Trivial => fun body_tp body t pf => body t
-    | _ => fun body_tp body t pf => body t pf
-  end.
-
-(* The type of Curried functions on the ops of spec *)
-Fixpoint ForallOps spec : (spec_ops spec -> Type) -> Type :=
-  match spec with
-    | Spec_Axioms _ => fun body_tp => body_tp tt
-    | Spec_ConsOp f T oppred rest =>
-      fun body_tp =>
-        ForallOp T oppred
-                 (fun t pf => ForallOps (rest t pf)
-                                        (fun ops => body_tp (ops_cons t pf ops)))
-  end.
-
-(* The type of Curried predicates on the ops of spec *)
-Definition OpsPred spec : Type := ForallOps spec (fun _ => Prop).
-
-(* Build a ForallOps function *)
-Fixpoint LambdaOps spec : forall body_tp, (forall ops, body_tp ops) ->
-                                          ForallOps spec body_tp :=
-  match spec return forall body_tp, (forall ops, body_tp ops) ->
-                                    ForallOps spec body_tp with
-    | Spec_Axioms _ =>
-      fun body_tp body => body tt
-    | Spec_ConsOp f T oppred rest =>
-      fun body_tp body =>
-        LambdaOp T oppred _
-                 (fun t pf =>
-                    LambdaOps (rest t pf) _ (fun ops => body (ops_cons t pf ops)))
-  end.
-
-(* Replace all the trivial True proofs in a spec_ops with I *)
-Fixpoint replace_op_proofs spec : spec_ops spec -> spec_ops spec :=
-  match spec with
-    | Spec_Axioms _ => fun ops => ops
-    | Spec_ConsOp f T oppred rest =>
-      fun ops =>
-        ops_cons (ops_head ops)
-                 (replace_op_proof T oppred _ (ops_proof ops))
-                 (replace_op_proofs (rest _ _)
-                                    (rew [fun pf => spec_ops (rest _ pf)]
-                                         replace_op_proof_eq T oppred _ _
-                                         in (ops_rest ops)))
-  end.
-
-(* Replacing all the trivial proofs yields an equal ops list *)
-Lemma replace_op_proofs_eq spec ops : replace_op_proofs spec ops = ops.
-  induction spec.
-  reflexivity.
-  unfold replace_op_proofs; fold replace_op_proofs.
-  destruct ops as [t ops]; destruct ops as [pf ops].
-  unfold ops_head; unfold ops_proof; unfold ops_rest; unfold ops_cons;
-    unfold projT1; unfold projT2.
-  destruct oppred; unfold replace_op_proof; unfold replace_op_proof_eq;
-    rewrite H; unfold eq_rect;
-    [ destruct pf | | ]; reflexivity.
-Qed.
-
-(* Apply a Curried predicate to some candidate ops for spec *)
-Fixpoint ApplyOps spec : forall A, (ForallOps spec A) ->
-                                   forall ops, A (replace_op_proofs spec ops) :=
-  match spec return forall A, (ForallOps spec A) ->
-                              forall ops, A (replace_op_proofs spec ops) with
-    | Spec_Axioms _ =>
-      fun A body ops => rew [A] (unit_eq _ _) in body
-    | Spec_ConsOp f T oppred rest =>
-      fun A body ops =>
-        ApplyOps
-          (rest (ops_head ops)
-                (replace_op_proof T oppred _ (ops_proof ops)))
-          (fun ops => A (ops_cons _ _ ops))
-          (ApplyOp T oppred _ body (ops_head ops) (ops_proof ops))
-          (rew [fun pf => spec_ops (rest _ pf)]
-               replace_op_proof_eq T oppred _ _ in ops_rest ops)
-  end.
-
-
-(*** Types / Typeclasses Represented by Specs ***)
-
-(* FIXME: remove IsoToSpec and IsoInterpretation, and possibly ForallOps *)
-
-(* Whether P is isomorphic to spec *)
-Class IsoToSpec spec (P: OpsPred spec) : Prop :=
-  spec_iso: forall ops, ApplyOps spec _ P ops <-> spec_model spec ops.
-
-(* An IsoInterpretation is an interpretation between type classes / type
-functions that are isomorphic to specs *)
-Definition IsoInterpretation {spec1 P1} (iso1: IsoToSpec spec1 P1)
-           {spec2 P2} (iso2: IsoToSpec spec2 P2)
-           (ops_f: spec_ops spec2 -> spec_ops spec1) : Type :=
-  ForallOps spec2 (fun ops2 => ApplyOps spec2 _ P2 ops2 ->
-                               ApplyOps spec1 _ P1 (ops_f ops2)).
-
-(* Turn an interpretation from spec1 to spec2 into a function from a predicate
-isomorphic to spec2 to a predicate ismorphic to spec1 *)
-Definition toIsoInterp {spec1 P1} {iso1: IsoToSpec spec1 P1}
-           {spec2 P2} {iso2: IsoToSpec spec2 P2}
-           (i: Interpretation spec1 spec2) :
-  IsoInterpretation iso1 iso2 (map_ops i) :=
-  LambdaOps spec2 _ (fun ops2 p2 =>
-                       proj2 (spec_iso (map_ops i ops2))
-                             (map_model i ops2 (proj1 (spec_iso ops2) p2))).
-
-(* Turn an IsoInterpretation into an Interpretation *)
-Definition fromIsoInterp {spec1 P1} {iso1: IsoToSpec spec1 P1}
-           {spec2 P2} {iso2: IsoToSpec spec2 P2} {ops_f}
-           (i: IsoInterpretation iso1 iso2 ops_f) :
-  Interpretation spec1 spec2 :=
-  mkInterp ops_f (fun ops2 model2 =>
-                    proj1 (spec_iso (ops_f ops2))
-                          (rew [fun ops => ApplyOps spec1 _ P1 (ops_f ops)]
-                               (replace_op_proofs_eq _ _)
-                            in ApplyOps _ _ i ops2
-                                        (rew [ApplyOps spec2 _ P2]
-                                             (eq_sym (replace_op_proofs_eq _ _))
-                                          in proj2 (spec_iso ops2) model2))).
-
-
-(*** Examples of Isomorphic Interpretations ***)
-
-(* Tactic to prove IsoToSpec instances *)
-Ltac prove_spec_iso :=
-  intro ops;
-  repeat (let t := fresh "t" in
-          let pf := fresh "pf" in
-          destruct ops as [t ops]; destruct ops as [pf ops];
-          try destruct pf);
-  destruct ops; split; compute;
-  [ intro H; destruct H;
-    repeat (first [ assumption | split; [assumption|] | apply I])
-  | intro H; repeat (let Hi := fresh "H" in
-                     destruct H as [Hi H]); constructor; assumption ].
-
-(* Example 1:  op n:nat;  axiom gt1: n > 1 *)
-Class spec_example_1_class (n:nat) : Prop :=
-  { example_1__gt1 : n > 1 }.
-
-(* Isomorphism between spec_example_1 and spec_example_1_class *)
-Instance iso_example_1 : IsoToSpec spec_example_1 spec_example_1_class.
-prove_spec_iso.
-Qed.
-
-(* Example 2:  op n:nat := 2;  (no axioms) *)
-Class spec_example_2_class (n:nat) (n__pf: n = 2) : Prop := { }.
-
-Instance iso_example_2 : IsoToSpec spec_example_2 spec_example_2_class.
-prove_spec_iso.
-Qed.
-
-(* Example 3:  op T:Set := nat;  op n:T__def;  axiom gt1: n > 1 *)
-Class spec_example_3_class (T:Set) (T__pf: T = nat) (n: def T T__pf) : Prop :=
-  { example_3__gt1 : n > 1 }.
-
-Instance iso_example_3 : IsoToSpec spec_example_3 spec_example_3_class.
-prove_spec_iso.
-Qed.
-
-(* Example: lift the spec3 -> spec2 interpretation to an instance function *)
-Instance iso_interp_example_3_2 : forall `{spec_example_2_class}, spec_example_3_class _ _ _ :=
-  toIsoInterp (interp_example_3_2).
-
-(* Example 4: monoids *)
-Class Monoid {T:Set} {m_zero:T} {m_plus:T -> T -> T} : Prop :=
-  {m_zero_left : (forall x, m_plus m_zero x = x);
-   m_zero_right : (forall x, m_plus x m_zero = x);
-   m_plus_assoc : (forall x y z, m_plus x (m_plus y z) = m_plus (m_plus x y) z)}.
-
-Instance iso_example_monoid : IsoToSpec spec_example_monoid (@Monoid).
-prove_spec_iso.
-Qed.
-
-(* Example 4: groups *)
-Class Group {T:Set} {g_zero:T} {g_plus:T -> T -> T} {g_inv:T -> T} : Prop :=
-  {g_zero_left : (forall x, g_plus g_zero x = x);
-   g_zero_right : (forall x, g_plus x g_zero = x);
-   g_plus_assoc : (forall x y z, g_plus x (g_plus y z) = g_plus (g_plus x y) z);
-   g_inv_left : (forall (x:T), g_plus (g_inv x) x = g_zero);
-   g_inv_right : (forall (x:T), g_plus x (g_inv x) = g_zero)}.
-
-Instance iso_example_group : IsoToSpec spec_example_group (@Group).
-prove_spec_iso.
-Qed.
-
-(* Interpretation from Monoid to Group type classes *)
-Program Instance group_as_monoid `{Group} :
-  Monoid (m_zero:=g_zero) (m_plus:=g_plus).
-Next Obligation. apply g_zero_left. Qed.
-Next Obligation. apply g_zero_right. Qed.
-Next Obligation. apply g_plus_assoc. Qed.
-
-(*
-NOTE: the below loops forever!
-
-Check (@group_as_monoid : IsoInterpretation iso_example_monoid iso_example_group _).
-Check (fromIsoInterp (iso1:=iso_example_monoid)
-                     (iso2:=iso_example_group)
-                     (@group_as_monoid)).
-*)
-
-
-(*** An Alternative Isomorphism to Specs ***)
-
-Class IsoToSpecModels {spec} (ops: spec_ops spec) (P: Prop) : Prop :=
-  spec_models_iso : P <-> spec_model spec ops.
-
-(* Tactic to prove IsoToSpec instances *)
-Ltac prove_spec_models_iso :=
-  split; compute;
-  [ intro H; destruct H;
-    repeat (first [ assumption | split; [assumption|] | apply I])
-  | intro H; repeat (let Hi := fresh "H" in
-                     destruct H as [Hi H]); constructor; assumption ].
+Class IsoToSpec spec (T:Type) : Type :=
+  {spec_iso1 : T -> spec_model spec;
+   spec_iso2 : spec_model spec -> T}.
 
 
 (*** Spec Translations ***)
@@ -1200,6 +773,8 @@ Notation "'{' '}'" :=
 Bind Scope spec_translation_scope with SpecTranslation.
 Delimit Scope spec_translation_scope with spec_translation.
 
+(* Translate a field using a single translation element, returning None if the
+translation element did not match the field *)
 Definition translate_field1 elem (f: Field) : option Field :=
   match elem with
     | XlateSingle f_from f_to =>
@@ -1211,6 +786,7 @@ Definition translate_field1 elem (f: Field) : option Field :=
       else None
   end.
 
+(* Translate a field *)
 Definition translate_field xlate f : Field :=
   match xlate with
     | mkSpecTranslation elems =>
@@ -1221,92 +797,41 @@ Definition translate_field xlate f : Field :=
                     end) f elems
   end.
 
-Definition translate_spec_axioms xlate axioms : list SpecAxiom :=
-  map (fun ax =>
-         match ax with
-           | specAxiom f P => specAxiom (translate_field xlate f) P
-         end) axioms.
-
+(* Translate all the fields in a spec *)
 Fixpoint translate_spec xlate spec : Spec :=
   match spec with
-    | Spec_Axioms axioms =>
-      Spec_Axioms (translate_spec_axioms xlate axioms)
-    | Spec_ConsOp f T oppred rest =>
-      Spec_ConsOp (translate_field xlate f) T oppred
-                  (fun x x__pf => translate_spec xlate (rest x x__pf))
+    | Spec_Nil => Spec_Nil
+    | Spec_Cons f T oppred rest =>
+      Spec_Cons (translate_field xlate f) T oppred
+                (fun x x__pf => translate_spec xlate (rest x x__pf))
   end.
 
-(* NOTE: the spec_ops type of a translated spec is in fact equal to that of the
-original spec, but this requires functional extensionality to prove... *)
+(* NOTE: the spec_model type of a translated spec is in fact equal to that of
+the original spec, but this requires functional extensionality to prove... *)
 
-Fixpoint translate_spec_ops xlate spec :
-  spec_ops (translate_spec xlate spec) -> spec_ops spec :=
-  match spec return spec_ops (translate_spec xlate spec) -> spec_ops spec with
-    | Spec_Axioms _ => fun ops => ops
-    | Spec_ConsOp f T oppred rest =>
-      fun ops =>
-        match ops with
-          | existT _ t_o (existT _ pf_o ops') =>
-            ops_cons t_o pf_o (translate_spec_ops xlate _ ops')
-        end
-  end.
-
-Lemma translate_spec_axioms_impl xlate axioms :
-  conjoin_axioms (translate_spec_axioms xlate axioms) -> conjoin_axioms axioms.
-  induction axioms.
-  intro; assumption.
-  destruct axioms; destruct a.
-  intro; assumption.
-  intro H; destruct H; split.
-  assumption.
-  apply IHaxioms; assumption.
-Defined.
-
-(* Build an interpretation from spec to (translate_spec xlate spec) *)
-Program Definition interp_translate_spec xlate spec :
+Fixpoint interp_translate_spec xlate spec :
   Interpretation spec (translate_spec xlate spec) :=
-  mkInterp (translate_spec_ops xlate spec) _.
-Next Obligation.
-revert ops H; induction spec; intros.
-apply (translate_spec_axioms_impl xlate); assumption.
-destruct ops as [t_o ops]; destruct ops as [pf_o ops].
-apply H. assumption.
-Defined.
-
-(* Reverse the translation of spec ops *)
-Fixpoint untranslate_spec_ops xlate spec :
-  spec_ops spec -> spec_ops (translate_spec xlate spec) :=
-  match spec return spec_ops spec -> spec_ops (translate_spec xlate spec) with
-    | Spec_Axioms _ => fun ops => ops
-    | Spec_ConsOp f T oppred rest =>
-      fun ops =>
-        match ops with
-          | existT _ t_o (existT _ pf_o ops') =>
-            ops_cons t_o pf_o (untranslate_spec_ops xlate _ ops')
+  match spec return Interpretation spec (translate_spec xlate spec) with
+    | Spec_Nil => fun model => model
+    | Spec_Cons f T oppred rest =>
+      fun model =>
+        match model with
+          | modelCons t pf model' =>
+            modelCons t pf (interp_translate_spec xlate _ model')
         end
   end.
 
-Lemma untranslate_spec_axioms_impl xlate axioms :
-  conjoin_axioms axioms -> conjoin_axioms (translate_spec_axioms xlate axioms).
-  induction axioms.
-  intro; assumption.
-  destruct axioms; destruct a.
-  intro; assumption.
-  intro H; destruct H; split.
-  assumption.
-  apply IHaxioms; assumption.
-Defined.
-
-(* Build an interpretation from (translate_spec xlate spec) back to spec *)
-Program Definition interp_untranslate_spec xlate spec :
+Fixpoint interp_untranslate_spec xlate spec :
   Interpretation (translate_spec xlate spec) spec :=
-  mkInterp (untranslate_spec_ops xlate spec) _.
-Next Obligation.
-revert ops H; induction spec; intros.
-apply (untranslate_spec_axioms_impl xlate); assumption.
-destruct ops as [t_o ops]; destruct ops as [pf_o ops].
-apply H. assumption.
-Defined.
+  match spec return Interpretation (translate_spec xlate spec) spec with
+    | Spec_Nil => fun model => model
+    | Spec_Cons f T oppred rest =>
+      fun model =>
+        match model with
+          | modelCons t pf model' =>
+            modelCons t pf (interp_untranslate_spec xlate _ model')
+        end
+  end.
 
 (* Translate an interpretation *)
 Definition translate_interp {spec1 spec2} xlate
@@ -1327,26 +852,12 @@ Definition interp_cons_strengthen_xlate xlate f1 T (oppred1 oppred2: OpPred T)
            (impl: forall t, oppred2 t -> oppred1 t)
            (i: forall t pf2,
                  Interpretation (spec1 t (impl t pf2)) (spec2 t pf2)) :
-  Interpretation (Spec_ConsOp f1 T oppred1 spec1)
-                 (Spec_ConsOp (translate_field xlate f1) T oppred2 spec2) :=
-  mkInterp (fun ops2:spec_ops (Spec_ConsOp (translate_field xlate f1)
-                                           T oppred2 spec2) =>
-              let (t_o,o) := ops2 in
-              let (pf_o, rest_o) := o in
-              ops_cons t_o (impl _ pf_o) (map_ops (i t_o pf_o) rest_o))
-           (fun ops2 =>
-              match ops2
-                    return spec_model (Spec_ConsOp (translate_field xlate f1)
-                                                   T oppred2 spec2) ops2 ->
-                           spec_model
-                             (Spec_ConsOp f1 T oppred1 spec1)
-                             (let (t_o,o) := ops2 in
-                              let (pf_o,rest_o) := o in
-                              ops_cons t_o (impl t_o pf_o) (map_ops (i _ _) rest_o)) with
-                | existT _ t_o (existT _ pf_o rest_o) =>
-                  fun model2 =>
-                    map_model (i t_o pf_o) rest_o model2
-              end).
+  Interpretation (Spec_Cons f1 T oppred1 spec1)
+                 (Spec_Cons (translate_field xlate f1) T oppred2 spec2) :=
+  (fun model2:spec_model (Spec_Cons (translate_field xlate f1)
+                                T oppred2 spec2) =>
+     let (t,pf,rest_m) := model2 in
+     modelCons t (impl _ pf) (i t pf rest_m)).
 
 (* Similar to the above, but substitute the definition of an op that is defined
 in the co-domain into the domain spec *)
@@ -1355,26 +866,12 @@ Definition interp_cons_def_xlate xlate f1 T (oppred1: OpPred T) t2
            (oppred1_pf: oppred1 t2)
            (i: forall t pf2,
                  Interpretation (spec1 t2 oppred1_pf) (spec2 t pf2)) :
-  Interpretation (Spec_ConsOp f1 T oppred1 spec1)
-                 (Spec_ConsOp (translate_field xlate f1) T (Pred_Eq t2) spec2) :=
-  mkInterp (fun ops2:spec_ops (Spec_ConsOp (translate_field xlate f1)
-                                           T (Pred_Eq t2) spec2) =>
-              let (t_o,o) := ops2 in
-              let (pf_o, rest_o) := o in
-              ops_cons t2 oppred1_pf (map_ops (i t_o pf_o) rest_o))
-           (fun ops2 =>
-              match ops2
-                    return spec_model (Spec_ConsOp (translate_field xlate f1)
-                                                   T (Pred_Eq t2) spec2) ops2 ->
-                           spec_model
-                             (Spec_ConsOp f1 T oppred1 spec1)
-                             (let (t_o,o) := ops2 in
-                              let (pf_o,rest_o) := o in
-                              ops_cons t2 oppred1_pf (map_ops (i _ _) rest_o)) with
-                | existT _ t_o (existT _ pf_o rest_o) =>
-                  fun model2 =>
-                    map_model (i t_o pf_o) rest_o model2
-              end).
+  Interpretation (Spec_Cons f1 T oppred1 spec1)
+                 (Spec_Cons (translate_field xlate f1) T (Pred_Eq t2) spec2) :=
+  (fun model2:spec_model (Spec_Cons (translate_field xlate f1)
+                                T (Pred_Eq t2) spec2) =>
+     let (t,pf,rest_m) := model2 in
+     modelCons t2 oppred1_pf (i t pf rest_m)).
 
 (* Similar to the above, but allow the field types to be provably, not just
 definitionally, equal *)
@@ -1384,26 +881,12 @@ Definition interp_cons_strengthen_xlate_eq xlate f1 T1 T2 (oppred1: OpPred T1)
            (eT: T2 = T1) (impl: forall t, oppred2 t -> oppred1 (rew eT in t))
            (i: forall t pf2,
                  Interpretation (spec1 (rew eT in t) (impl t pf2)) (spec2 t pf2)) :
-  Interpretation (Spec_ConsOp f1 T1 oppred1 spec1)
-                 (Spec_ConsOp (translate_field xlate f1) T2 oppred2 spec2) :=
-  mkInterp (fun ops2:spec_ops (Spec_ConsOp (translate_field xlate f1)
-                                           T2 oppred2 spec2) =>
-              let (t_o,o) := ops2 in
-              let (pf_o, rest_o) := o in
-              ops_cons (rew eT in t_o) (impl _ pf_o) (map_ops (i t_o pf_o) rest_o))
-           (fun ops2 =>
-              match ops2
-                    return spec_model (Spec_ConsOp (translate_field xlate f1)
-                                                   T2 oppred2 spec2) ops2 ->
-                           spec_model
-                             (Spec_ConsOp f1 T1 oppred1 spec1)
-                             (let (t_o,o) := ops2 in
-                              let (pf_o,rest_o) := o in
-                              ops_cons (rew eT in t_o) (impl t_o pf_o) (map_ops (i _ _) rest_o)) with
-                | existT _ t_o (existT _ pf_o rest_o) =>
-                  fun model2 =>
-                    map_model (i t_o pf_o) rest_o model2
-              end).
+  Interpretation (Spec_Cons f1 T1 oppred1 spec1)
+                 (Spec_Cons (translate_field xlate f1) T2 oppred2 spec2) :=
+  (fun model2:spec_model (Spec_Cons (translate_field xlate f1)
+                                T2 oppred2 spec2) =>
+     let (t,pf,rest_m) := model2 in
+     modelCons (rew eT in t) (impl _ pf) (i t pf rest_m)).
 
 (* Tactic to prove a "simple" interpretation, which is one where none of the ops
 have to be re-ordered, but where the fields can be translated between the domain
@@ -1424,8 +907,8 @@ Ltac intros_for_cons_op f oppred :=
 Ltac prove_simple_interp xlate :=
   let next :=
       lazymatch goal with
-      | |- Interpretation (Spec_ConsOp ?f1 ?T1 ?oppred1 ?rest1)
-                          (Spec_ConsOp ?f2 ?T2 ?oppred2 ?rest2) =>
+      | |- Interpretation (Spec_Cons ?f1 ?T1 ?oppred1 ?rest1)
+                          (Spec_Cons ?f2 ?T2 ?oppred2 ?rest2) =>
         lazymatch (eval cbn in (Field_dec f2 (translate_field xlate f1))) with
           | left _ =>
             first
@@ -1442,19 +925,10 @@ Ltac prove_simple_interp xlate :=
           | right _ =>
             apply interp_cons_r; intros; prove_simple_interp xlate
         end
-      | |- Interpretation (Spec_Axioms _)
-                          (Spec_ConsOp ?f2 ?T2 ?oppred2 ?rest2) =>
-        apply interp_cons_r; intros_for_cons_op f2 oppred2;
-        prove_simple_interp xlate
-      | |- Interpretation (Spec_Axioms _) (Spec_Axioms _) =>
-        idtac "axioms";
-        apply (mkInterp (fun _ => tt : spec_ops (Spec_Axioms _)));
-        intros ops model; unfold spec_model, conjoin_axioms in model;
-        repeat (let ax_name := fresh "axiom" in
-                first [ destruct model as [ax_name model]
-                      | rename model into ax_name ]);
-        unfold spec_model, conjoin_axioms; repeat split;
-        try assumption
+      | |- Interpretation Spec_Nil (Spec_Cons ?f2 ?T2 ?oppred2 ?rest2) =>
+        apply interp_cons_r; intros; prove_simple_interp xlate
+      | |- Interpretation Spec_Nil Spec_Nil =>
+        apply (fun _ => tt : spec_model Spec_Nil)
       | |- Interpretation ?S1 ?S2 =>
         let S1' := (eval hnf in S1) in
         let S2' := (eval hnf in S2) in
@@ -1466,22 +940,9 @@ Ltac prove_simple_interp xlate :=
       next
 .
 
-(* Old version *)
-(*
-Ltac prove_simple_interp xlate :=
-  repeat (first [apply (interp_cons_strengthen_xlate xlate);
-                  intros; [ try assumption | ]
-                | apply interp_cons_r; intros ]);
-  apply (mkInterp (fun _ => tt : spec_ops (Spec_Axioms _))); intros ops model;
-  unfold spec_model, conjoin_axioms, specAxiom, snd in model;
-  repeat (let ax_name := fresh "axiom" in
-          first [ destruct model as [ax_name model] | rename model into ax_name ]);
-  unfold spec_model, conjoin_axioms, specAxiom, snd; repeat split;
-  try assumption.
-*)
-
 
 (* For proving the model part of an interpretation given by an interp_map *)
+(*
 Ltac interp_tactic :=
   intros;
   lazymatch goal with
@@ -1491,12 +952,10 @@ Ltac interp_tactic :=
     | |- Pred_Fun _ => try assumption
     | |- _ => try (apply I); try assumption
   end.
+*)
 
 
 (*** Refinement ***)
-
-(* Helper wrapper around the refine tactic *)
-Ltac specware_refine arg := refine arg.
 
 (* A refinement import into spec is some spec', an interpretation from spec' to
 spec, and a type that is isomorphic to spec' *)
